lean/TSLean/JS/AxiomAudit.lean
@@ -4,6 +4,7 @@ import TSLean.JS.AbstractOperationTheorems
 import TSLean.JS.ExecutionTheorems
 import TSLean.JS.FunctionTheorems
 import TSLean.JS.HeapTheorems
+import TSLean.JS.OrderedProps
 import TSLean.JS.PrimitiveTheorems
 
 #audit_proofs TSLean.JS
